opentheory/examples/word.ml
@@ -5,16 +5,28 @@
 logfile "list-interval-def";;
 
 let interval_def = new_recursive_definition num_RECURSION
-  `(interval m 0 = []) /\
-   (interval m (SUC n) = CONS m (interval (SUC m) n))`;;
+  `(!m. interval m 0 = []) /\
+   (!m n. interval m (SUC n) = CONS m (interval (SUC m) n))`;;
 
 export_thm interval_def;;
+
+logfile "list-interval-thm";;
+
+let length_interval = prove
+  (`!m n. LENGTH (interval m n) = n`,
+   ONCE_REWRITE_TAC [SWAP_FORALL_THM] THEN
+   MATCH_MP_TAC num_INDUCTION THEN
+   SIMP_TAC [LENGTH; interval_def; SUC_INJ]);;
+
+export_thm length_interval;;
 
 logfile "list-zipwith-def";;
 
 let zipwith_raw_def = new_recursive_definition list_RECURSION
-  `(zipwith f [] l = []) /\
-   (zipwith f (CONS h t) l = CONS (f h (HD l)) (zipwith f t (TL l)))`;;
+  `(!f l. zipwith f [] l = []) /\
+   (!f h t l.
+      zipwith f (CONS h t) l =
+      CONS (f h (HD l)) (zipwith f t (TL l)))`;;
 
 let zipwith_def = prove
    (`(!f. zipwith (f : A -> B -> C) [] [] = []) /\
@@ -24,6 +36,23 @@ let zipwith_def = prove
     REWRITE_TAC [zipwith_raw_def; HD; TL]);;
 
 export_thm zipwith_def;;
+
+logfile "list-zipwith-thm";;
+
+let length_zipwith = prove
+  (`!(f : A -> B -> C) l1 l2 n.
+      LENGTH l1 = n /\ LENGTH l2 = n ==> LENGTH (zipwith f l1 l2) = n`,
+   GEN_TAC THEN
+   LIST_INDUCT_TAC THEN
+   LIST_INDUCT_TAC THEN
+   ASM_SIMP_TAC [LENGTH; zipwith_def] THEN
+   GEN_TAC THEN
+   MP_TAC (SPEC `n:num` num_CASES) THEN
+   STRIP_TAC THEN
+   ASM_SIMP_TAC [NOT_SUC; SUC_INJ] THEN
+   FIRST_ASSUM MATCH_ACCEPT_TAC);;
+
+export_thm length_zipwith;;
 
 new_constant ("word_width", `:num`);;
 
@@ -54,50 +83,80 @@ new_constant ("word_lt", `:word -> word -> bool`);;
 new_constant ("num_to_word", `:num -> word`);;
 new_constant ("word_to_num", `:word -> num`);;
 
+let word_to_num_from_num = new_axiom
+  `!x. num_to_word (word_to_num x) = x`;;
+
+let num_to_word_inj = new_axiom
+  `!x y. x < word_size /\ y < word_size /\ num_to_word x = num_to_word y ==> x = y`;;
+
+let num_to_word_to_num = new_axiom
+  `!x. word_to_num (num_to_word x) = x MOD word_size`;;
+
+let num_to_word_add = new_axiom
+  `!x1 y1. num_to_word (x1 + y1) = word_add (num_to_word x1) (num_to_word y1)`;;
+
+let num_to_word_mult = new_axiom
+  `!x1 y1. num_to_word (x1 * y1) = word_mult (num_to_word x1) (num_to_word y1)`;;
+
+let word_neg_def = new_axiom
+  `!x. word_neg x = num_to_word (word_size - word_to_num x)`;;
+
+let word_sub_def = new_axiom
+  `!x y. word_sub x y = word_add x (word_neg y)`;;
+
+let word_le_def = new_axiom
+  `!x y. word_le x y = word_to_num x <= word_to_num y`;;
+
+let word_lt_def = new_axiom
+  `!x y. word_lt x y = ~(word_le y x)`;;
+
 logfile "word-bits";;
 
 let word_shl_def = new_definition
- `word_shl w n = num_to_word (word_to_num w * (2 EXP n))`;;
+ `!w n. word_shl w n = num_to_word (word_to_num w * (2 EXP n))`;;
 
 export_thm word_shl_def;;
 
 let word_shr_def = new_definition
- `word_shr w n = num_to_word (word_to_num w DIV (2 EXP n))`;;
+ `!w n. word_shr w n = num_to_word (word_to_num w DIV (2 EXP n))`;;
 
 export_thm word_shr_def;;
 
 let word_bit_def = new_definition
- `word_bit w n = ODD (word_to_num (word_shr w n))`;;
+ `!w n. word_bit w n = ODD (word_to_num (word_shr w n))`;;
 
 export_thm word_bit_def;;
 
 let word_to_list_def = new_definition
- `word_to_list w = MAP (word_bit w) (interval 0 word_width)`;;
+ `!w. word_to_list w = MAP (word_bit w) (interval 0 word_width)`;;
 
 export_thm word_to_list_def;;
 
 let list_to_word_def = new_recursive_definition list_RECURSION
   `(list_to_word [] = num_to_word 0) /\
-   (list_to_word (CONS h t) =
-    if h then word_add (word_shl (list_to_word t) 1) (num_to_word 1)
-    else word_shl (list_to_word t) 1)`;;
+   (!h t.
+      list_to_word (CONS h t) =
+      if h then word_add (word_shl (list_to_word t) 1) (num_to_word 1)
+      else word_shl (list_to_word t) 1)`;;
 
 export_thm list_to_word_def;;
 
 let word_and_def = new_definition
-  `word_and w1 w2 =
-   list_to_word (zipwith ( /\ ) (word_to_list w1) (word_to_list w2))`;;
+  `!w1 w2.
+     word_and w1 w2 =
+     list_to_word (zipwith ( /\ ) (word_to_list w1) (word_to_list w2))`;;
 
 export_thm word_and_def;;
 
 let word_or_def = new_definition
-  `word_or w1 w2 =
-   list_to_word (zipwith ( \/ ) (word_to_list w1) (word_to_list w2))`;;
+  `!w1 w2.
+     word_or w1 w2 =
+     list_to_word (zipwith ( \/ ) (word_to_list w1) (word_to_list w2))`;;
 
 export_thm word_or_def;;
 
 let word_not_def = new_definition
-  `word_not w = list_to_word (MAP (~) (word_to_list w))`;;
+  `!w. word_not w = list_to_word (MAP (~) (word_to_list w))`;;
 
 export_thm word_not_def;;
 
