opentheory/examples/byte.ml
@@ -32,3 +32,70 @@ new_constant ("byte_shr", `:byte -> num -> byte`);;
 new_constant ("byte_size", `:num`);;
 new_constant ("byte_to_list", `:byte -> bool list`);;
 new_constant ("byte_to_num", `:byte -> num`);;
+
+let byte_size_def = new_axiom
+  `byte_size = 2 EXP byte_width`;;
+
+let byte_size_nonzero = new_axiom
+  `~(byte_size = 0)`;;
+
+let byte_to_num_from_num = new_axiom
+  `!x. num_to_byte (byte_to_num x) = x`;;
+
+let num_to_byte_inj = new_axiom
+  `!x y. x < byte_size /\ y < byte_size /\ num_to_byte x = num_to_byte y ==> x = y`;;
+
+let num_to_byte_to_num = new_axiom
+  `!x. byte_to_num (num_to_byte x) = x MOD byte_size`;;
+
+let num_to_byte_add = new_axiom
+  `!x1 y1. num_to_byte (x1 + y1) = byte_add (num_to_byte x1) (num_to_byte y1)`;;
+
+let num_to_byte_mult = new_axiom
+  `!x1 y1. num_to_byte (x1 * y1) = byte_mult (num_to_byte x1) (num_to_byte y1)`;;
+
+let byte_neg_def = new_axiom
+  `!x. byte_neg x = num_to_byte (byte_size - byte_to_num x)`;;
+
+let byte_sub_def = new_axiom
+  `!x y. byte_sub x y = byte_add x (byte_neg y)`;;
+
+let byte_le_def = new_axiom
+  `!x y. byte_le x y = byte_to_num x <= byte_to_num y`;;
+
+let byte_lt_def = new_axiom
+  `!x y. byte_lt x y = ~(byte_le y x)`;;
+
+let byte_shl_def = new_axiom
+ `!w n. byte_shl w n = num_to_byte (byte_to_num w * (2 EXP n))`;;
+
+let byte_shr_def = new_axiom
+ `!w n. byte_shr w n = num_to_byte (byte_to_num w DIV (2 EXP n))`;;
+
+let byte_bit_def = new_axiom
+ `!w n. byte_bit w n = ODD (byte_to_num (byte_shr w n))`;;
+
+let byte_to_list_def = new_axiom
+ `!w. byte_to_list w = MAP (byte_bit w) (interval 0 byte_width)`;;
+
+let list_to_byte_def = new_axiom
+  `(list_to_byte [] = num_to_byte 0) /\
+   (!h t.
+      list_to_byte (CONS h t) =
+      if h then byte_add (byte_shl (list_to_byte t) 1) (num_to_byte 1)
+      else byte_shl (list_to_byte t) 1)`;;
+
+let byte_and_def = new_axiom
+  `!w1 w2.
+     byte_and w1 w2 =
+     list_to_byte (zipwith ( /\ ) (byte_to_list w1) (byte_to_list w2))`;;
+
+let byte_or_def = new_axiom
+  `!w1 w2.
+     byte_or w1 w2 =
+     list_to_byte (zipwith ( \/ ) (byte_to_list w1) (byte_to_list w2))`;;
+
+let byte_not_def = new_axiom
+  `!w. byte_not w = list_to_byte (MAP (~) (byte_to_list w))`;;
+
+logfile_end ();;
