opentheory/examples/word16.ml
@@ -33,17 +33,84 @@ new_constant ("word16_size", `:num`);;
 new_constant ("word16_to_list", `:word16 -> bool list`);;
 new_constant ("word16_to_num", `:word16 -> num`);;
 
+let word16_size_def = new_axiom
+  `word16_size = 2 EXP word16_width`;;
+
+let word16_size_nonzero = new_axiom
+  `~(word16_size = 0)`;;
+
+let word16_to_num_from_num = new_axiom
+  `!x. num_to_word16 (word16_to_num x) = x`;;
+
+let num_to_word16_inj = new_axiom
+  `!x y. x < word16_size /\ y < word16_size /\ num_to_word16 x = num_to_word16 y ==> x = y`;;
+
+let num_to_word16_to_num = new_axiom
+  `!x. word16_to_num (num_to_word16 x) = x MOD word16_size`;;
+
+let num_to_word16_add = new_axiom
+  `!x1 y1. num_to_word16 (x1 + y1) = word16_add (num_to_word16 x1) (num_to_word16 y1)`;;
+
+let num_to_word16_mult = new_axiom
+  `!x1 y1. num_to_word16 (x1 * y1) = word16_mult (num_to_word16 x1) (num_to_word16 y1)`;;
+
+let word16_neg_def = new_axiom
+  `!x. word16_neg x = num_to_word16 (word16_size - word16_to_num x)`;;
+
+let word16_sub_def = new_axiom
+  `!x y. word16_sub x y = word16_add x (word16_neg y)`;;
+
+let word16_le_def = new_axiom
+  `!x y. word16_le x y = word16_to_num x <= word16_to_num y`;;
+
+let word16_lt_def = new_axiom
+  `!x y. word16_lt x y = ~(word16_le y x)`;;
+
+let word16_shl_def = new_axiom
+ `!w n. word16_shl w n = num_to_word16 (word16_to_num w * (2 EXP n))`;;
+
+let word16_shr_def = new_axiom
+ `!w n. word16_shr w n = num_to_word16 (word16_to_num w DIV (2 EXP n))`;;
+
+let word16_bit_def = new_axiom
+ `!w n. word16_bit w n = ODD (word16_to_num (word16_shr w n))`;;
+
+let word16_to_list_def = new_axiom
+ `!w. word16_to_list w = MAP (word16_bit w) (interval 0 word16_width)`;;
+
+let list_to_word16_def = new_axiom
+  `(list_to_word16 [] = num_to_word16 0) /\
+   (!h t.
+      list_to_word16 (CONS h t) =
+      if h then word16_add (word16_shl (list_to_word16 t) 1) (num_to_word16 1)
+      else word16_shl (list_to_word16 t) 1)`;;
+
+let word16_and_def = new_axiom
+  `!w1 w2.
+     word16_and w1 w2 =
+     list_to_word16 (zipwith ( /\ ) (word16_to_list w1) (word16_to_list w2))`;;
+
+let word16_or_def = new_axiom
+  `!w1 w2.
+     word16_or w1 w2 =
+     list_to_word16 (zipwith ( \/ ) (word16_to_list w1) (word16_to_list w2))`;;
+
+let word16_not_def = new_axiom
+  `!w. word16_not w = list_to_word16 (MAP (~) (word16_to_list w))`;;
+
 logfile "word16-bytes";;
 
 let word16_to_bytes_def = new_definition
-  `word16_to_bytes w =
+  `!w.
+     word16_to_bytes w =
      (num_to_byte (word16_to_num (word16_shr w 8)),
       num_to_byte (word16_to_num (word16_and w (num_to_word16 255))))`;;
 
 export_thm word16_to_bytes_def;;
 
 let bytes_to_word16_def = new_definition
-  `bytes_to_word16 b1 b2 =
+  `!b1 b2.
+     bytes_to_word16 b1 b2 =
      word16_or
        (word16_shl (num_to_word16 (byte_to_num b1)) 8)
        (num_to_word16 (byte_to_num b2))`;;
